maybe it's a nice idea to write exactly what I was changing, no?

code/experimental/P256/Hacl.Impl.ECDSA.P256SHA256.Common.fst
@@ -1,31 +1,24 @@
-
 module Hacl.Impl.ECDSA.P256SHA256.Common
 
 open FStar.HyperStack.All
 open FStar.HyperStack
 module ST = FStar.HyperStack.ST
 
-open Lib.IntTypes
 open Lib.Buffer
+open Lib.IntTypes
+open Lib.ByteBuffer 
+open Lib.ByteSequence
 
+open Hacl.Spec.P256 
 open Hacl.Spec.P256.Definitions
-open Hacl.Impl.LowLevel
-open Hacl.Impl.P256
-open Hacl.Spec.P256.MontgomeryMultiplication
-open Hacl.Impl.ECDSA.MontgomeryMultiplication
-open Hacl.Impl.ECDSA.MM.Exponent
 
 open Hacl.Spec.ECDSAP256.Definition
-open Hacl.Spec.ECDSA
-open Hacl.Spec.P256 
-open Hacl.Spec.P256.Ladder
-open Hacl.Spec.P256.Lemmas
 
-open Hacl.Impl.P256.PointAdd
-open Hacl.Impl.P256.LowLevel
+open Hacl.Impl.LowLevel
+open Hacl.Impl.ECDSA.MontgomeryMultiplication
 
-open Hacl.Hash.SHA2
 
+#set-options "--z3rlimit 100"
 
 val changeEndian: i: felem -> Stack unit 
   (requires fun h -> live h i)
@@ -42,45 +35,46 @@ let changeEndian i =
   upd i (size 3) zero
 
 
-
-open Lib.ByteBuffer 
-
-
 val toUint64ChangeEndian: i: lbuffer uint8 (32ul) -> o: felem ->  Stack unit
   (requires fun h -> live h i /\ live h o /\ disjoint i o)
-  (ensures fun h0 _ h1 -> modifies (loc o) h0 h1 
-    /\ as_seq h1 o == Hacl.Spec.ECDSA.changeEndian(Lib.ByteSequence.uints_from_bytes_be #_ #_ #4 (as_seq h0 i))
-   )
+  (ensures fun h0 _ h1 -> 
+    modifies (loc o) h0 h1 /\ 
+    as_seq h1 o == Hacl.Spec.ECDSA.changeEndian(Lib.ByteSequence.uints_from_bytes_be #_ #_ #4 (as_seq h0 i))
+  )
 
 let toUint64ChangeEndian i o = 
-  uints_from_bytes_be o i;
+  Lib.ByteBuffer.uints_from_bytes_be o i;
   changeEndian o
 
 
+inline_for_extraction noextract
 val toUint64: i: lbuffer uint8 (32ul) -> o: felem -> Stack unit
   (requires fun h -> live h i /\ live h o /\ disjoint i o)
-  (ensures 
-    fun h0 _ h1 -> modifies (loc o) h0 h1 /\ 
-      as_seq h1 o == Lib.ByteSequence.uints_from_bytes_le (as_seq h0 i))
+  (ensures fun h0 _ h1 -> 
+    modifies (loc o) h0 h1 /\ 
+    as_seq h1 o == Lib.ByteSequence.uints_from_bytes_le (as_seq h0 i)
+  )
 
 let toUint64 i o = 
-    Lib.ByteBuffer.uints_from_bytes_le o i
+  Lib.ByteBuffer.uints_from_bytes_le o i
 
 
+inline_for_extraction noextract
 val toUint8: i: felem ->  o: lbuffer uint8 (32ul) -> Stack unit
   (requires fun h -> live h i /\ live h o /\ disjoint i o)
-  (ensures fun h0 _ h1 -> modifies (loc o) h0 h1 /\ 
-    as_seq h1 o == Lib.ByteSequence.uints_to_bytes_le #_ #_ #4 (as_seq h0 i))
+  (ensures fun h0 _ h1 -> 
+    modifies (loc o) h0 h1 /\ 
+    as_seq h1 o == Lib.ByteSequence.uints_to_bytes_le #_ #_ #4 (as_seq h0 i)
+  )
 
 let toUint8 i o = 
-  uints_to_bytes_le (size 4) o i
-
+  Lib.ByteBuffer.uints_to_bytes_le (size 4) o i
 
 
 inline_for_extraction noextract
 val equalZeroBuffer: f: felem -> Stack bool
   (requires fun h -> live h f)
-  (ensures fun h0 r h1 -> modifies0 h0 h1 /\ (if as_nat h0 f = 0 then r == true else r == false ))
+  (ensures fun h0 r h1 -> modifies0 h0 h1 /\ (if as_nat h0 f = 0 then r == true else r == false))
 
 let equalZeroBuffer f =        
     let f0 = index f (size 0) in  
@@ -96,7 +90,6 @@ let equalZeroBuffer f =
     z0_zero && z1_zero && z2_zero && z3_zero
   
 
-
 (* checks whether the intefer f is between 1 and (n- 1) (incl).  *)
 (* [1, n - 1] <==> a > 0 /\ a < n) *)
 
@@ -110,57 +103,39 @@ val isMoreThanZeroLessThanOrderMinusOne: f: felem -> Stack bool
 
 let isMoreThanZeroLessThanOrderMinusOne f = 
   push_frame();
-    let h0 = ST.get() in 
     let tempBuffer = create (size 4) (u64 0) in 
         recall_contents prime256order_buffer (Lib.Sequence.of_list p256_order_prime_list);
-  let h0 = ST.get() in 
     let carry = sub4_il f prime256order_buffer tempBuffer in  
-      assert(if uint_v carry = 1 then as_nat h0 f < prime_p256_order else True);
-  let h1 = ST.get() in 
-  assert(modifies1 tempBuffer h0 h1);
     let less = eq_u64 carry (u64 1) in
-      assert(less == true ==> as_nat h0 f < prime_p256_order);
-  let h2 = ST.get() in 
     let more = equalZeroBuffer f in 
-      assert(not more == true ==> as_nat h0 f > 0);
-    let result = less &&  not more in 
-      assert(less && not more ==> as_nat h0 f > 0 && as_nat h0 f < prime_p256_order);
+    let result = less && not more in 
   pop_frame();  
     result
 
 
-val lemma_core_0: a: lbuffer uint64 (size 4) -> h: mem -> 
-  Lemma (Lib.ByteSequence.nat_from_intseq_le (as_seq h a) == as_nat h a)
+val lemma_core_0: a: lbuffer uint64 (size 4) -> h: mem -> Lemma (nat_from_intseq_le (as_seq h a) == as_nat h a)
 
 let lemma_core_0 a h = 
-  let open Lib.ByteSequence in 
-  
-    let k = as_seq h a in 
-    let z = nat_from_intseq_le k in 
-    
+  let k = as_seq h a in 
+  let z = nat_from_intseq_le k in 
     nat_from_intseq_le_slice_lemma k 1;
     nat_from_intseq_le_lemma0 (Seq.slice k 0 1);
-
-    let k1 = Seq.slice k 1 4 in 
-      nat_from_intseq_le_slice_lemma #_ #_ #3 k1 1;
-      nat_from_intseq_le_lemma0 (Seq.slice k1 0 1);
-      
-    let k2 = Seq.slice k1 1 3 in 
-      nat_from_intseq_le_slice_lemma #_ #_ #2 k2 1;
-      nat_from_intseq_le_lemma0 (Seq.slice k2 0 1);
-      nat_from_intseq_le_lemma0 (Seq.slice k2 1 2)
+  let k1 = Seq.slice k 1 4 in 
+    nat_from_intseq_le_slice_lemma #_ #_ #3 k1 1;
+    nat_from_intseq_le_lemma0 (Seq.slice k1 0 1);
+  let k2 = Seq.slice k1 1 3 in 
+    nat_from_intseq_le_slice_lemma #_ #_ #2 k2 1;
+    nat_from_intseq_le_lemma0 (Seq.slice k2 0 1);
+    nat_from_intseq_le_lemma0 (Seq.slice k2 1 2)
 
 
 val lemma_core_1: a: lbuffer uint64 (size 4) -> h: mem -> 
-  Lemma (Lib.ByteSequence.nat_from_bytes_le (Lib.ByteSequence.uints_to_bytes_le (as_seq h a)) == as_nat h a)
+  Lemma (nat_from_bytes_le (Lib.ByteSequence.uints_to_bytes_le (as_seq h a)) == as_nat h a)
 
 let lemma_core_1 a h= 
   let open Lib.ByteSequence in 
-  let k = as_seq h a in 
-  let z = Lib.ByteSequence.uints_to_bytes_le (as_seq h a) in 
-  let maint = Lib.ByteSequence.nat_from_bytes_le (Lib.ByteSequence.uints_to_bytes_le (as_seq h a)) in 
   lemma_core_0 a h;
   lemma_nat_from_to_intseq_le_preserves_value #U64 #SEC 4 (as_seq h a);
-  let n = nat_from_intseq_le k in 
+  let n = nat_from_intseq_le (as_seq h a) in 
   uints_to_bytes_le_nat_lemma #U64 #SEC 4 n;
   lemma_nat_to_from_bytes_le_preserves_value #SEC (uints_to_bytes_le #U64 #SEC #4 (as_seq h a)) 32 (as_nat h a)
